temp commit

ToCNF/IL.fst
@@ -1,126 +1,106 @@
 module IL
-	open FStar.Set
-	open FStar.Heap
-    open FStar.Map
 
-// Source
-//-----------------------------------------------------------------------------------------------------------------
-	type Position = {
-		absoluteOffset : int;
-		line: int;
-		column : int	
-	}
+type position = {
+    absoluteOffset : int;
+    line: int;
+    column : int	
+}
+assume HasEq_position: hasEq position
 
-	let new_position a l c = 
-		{absoluteOffset = a; line = l; column = c}
+let new_position a l c = {absoluteOffset = a; line = l; column = c}
 
-	type Source = {
-		text : string;
-		startPos : Position;
-		endPos : Position;
-		file : string
-	}
+type source = {
+    text : string;
+    startPos : position;
+    endPos : position;
+    file : string
+}
+assume HasEq_source: hasEq source
 
-    let new_Source t s e f = 
-		{text = t; startPos = s; endPos = e; file = f}
-		
-	(* (new_position 0 0 0) -- new Position()  :( *)
-	let new_Source0 text = new_Source text (new_position 0 0 0) (new_position 0 0 0) ""
-		
-//-----------------------------------------------------------------------------------------------------------------
+let new_Source t s e f = {text = t; startPos = s; endPos = e; file = f}
+	
+let new_Source0 text = new_Source text (new_position 0 0 0) (new_position 0 0 0) ""
 
-
-// Production
-//-----------------------------------------------------------------------------------------------------------------       
-    type DLabel = {
-        label: string;
-        weight: option float
-    }
+type dLabel = {
+    label: string;
+    weight: option int//float
+}
+assume HasEq_dLabel: hasEq dLabel
  
-    type elem 'patt 'expr = {
-        (*  Don't include rule into AST                                                                 *)
-        omit:bool;
-        (*  Production rule itself.                                                                     *)
-        rule:(Production 'patt 'expr);
-        (*  Binding :) like f:F or f:=F.... Seal                                                        *)
-        binding:option 'patt;
-        (*  Almost resolver (condition in production).                                                  *)
-        checker:option 'expr
-    }
-    (*  <summary>                                                                                       *)
-    (*  <para>t&lt;'patt,'expr&gt; - Type of production node in derivation tree. </para>                *)
-    (*  <para>  'patt - type of l-attributes. </para>                                                   *)
-    (*  <para>  'expr - type of expressions in action code. </para>                                     *)
-    (*  </summary>                                                                                      *)
-	and Production 'patt 'expr = 
-        (*  Alternative (e1 | e2)                                                                       *)
-        | PAlt     of (Production 'patt 'expr) * (Production 'patt 'expr)
-        (*  Sequence * attribute. (Attribute is always applied to sequence)                             *)
-        | PSeq     of list (elem 'patt 'expr)  * option 'expr * option DLabel
-        (*  Token itself. Final element of parsing.                                                     *)
-        | PToken   of Source
-        (*  Reference to other rule inside production. With an optional args list.                      *)
-        | PRef     of Source * option 'expr 
-        (*  expr*                                                                                       *)
-        | PMany    of (Production 'patt 'expr)
-        (*  Reference to metarule inside production (mr<<x>> in rule "a: mr<<x>> y z")                  *)
-        | PMetaRef of Source * (option 'expr) * list (Production 'patt 'expr) 
-        (*  Literal. We can use constants ("if" and "then" in ' .."if" expr "then" expr...')            *)
-        | PLiteral of Source 
-        (*  Extended regexp repetition, "man egrep" for details                                         *)
-        | PRepet   of (Production 'patt 'expr ) * (option int) * (option int) 
-        (*  Permutation (A || B || C)                                                                   *)
-        | PPerm    of list (Production 'patt 'expr) 
-        (*  The following are obsolete and reduction to PRepet should be discussed.                     *)
-        (*  expr+                                                                                       *)
-        | PSome    of (Production 'patt 'expr)
-        (*  expr?                                                                                       *)
-        | POpt     of (Production 'patt 'expr)  
+type elem 'patt 'expr = {
+    //Don't include rule into AST                                                                 
+    omit:bool;
+    //Production rule itself.                                                                     
+    rule:(production 'patt 'expr);
+    //Binding :) like f:F or f:=F.... Seal                                                        
+    binding:option 'patt;
+    //Almost resolver (condition in production).                                                  
+    checker:option 'expr
+}
 
-        (* with 																						*)
-        (* override this.ToString() = 																	*)
-//-----------------------------------------------------------------------------------------------------------------
+//'patt,'expr; - Type of production node in derivation tree.
+//'patt - type of l-attributes.
+//  'expr - type of expressions in action code.
+and production 'patt 'expr = 
+    (*  Alternative (e1 | e2)                                                                       *)
+    (*| PAlt     of (production 'patt 'expr) * (production 'patt 'expr)                             *)
+    (*  Sequence * attribute. (Attribute is always applied to sequence)                             *)
+    | PSeq     of list (elem 'patt 'expr)  * option 'expr * option dLabel
+    (*  Token itself. Final element of parsing.                                                     *)
+    | PToken   of source
+    (*  Reference to other rule inside production. With an optional args list.                      *)
+    | PRef     of source * option 'expr 
+    (*  expr*                                                                                       *)
+    (*| PMany    of (production 'patt 'expr)                                                        *)
+    (*  Reference to metarule inside production (mr<<x>> in rule "a: mr<<x>> y z")                  *)
+    (*| PMetaRef of source * (option 'expr) * list (production 'patt 'expr)                         *)
+    (*  Literal. We can use constants ("if" and "then" in ' .."if" expr "then" expr...')            *)
+    (*| PLiteral of source                                                                          *)
+    (*  Extended regexp repetition, "man egrep" for details                                         *)
+    (*| PRepet   of (production 'patt 'expr ) * (option int) * (option int)                         *)
+    (*  Permutation (A || B || C)                                                                   *)
+    (*| PPerm    of list (production 'patt 'expr)                                                   *)
+    (*  The following are obsolete and reduction to PRepet should be discussed.                     *)
+    (*  expr+                                                                                       *)
+    (*| PSome    of (production 'patt 'expr)                                                        *)
+    (*  expr?                                                                                       *)
+    (* | POpt     of (production 'patt 'expr)                                                       *)
+
+assume HasEq_elem: forall a b. hasEq a /\ hasEq b ==> hasEq (elem a b)
+assume HasEq_production: forall a b. hasEq a /\ hasEq b ==> hasEq (production a b)
 
 
-// Rule
-//-----------------------------------------------------------------------------------------------------------------
-    (*  <summary>                                                                                       *)
-    (*  <para>t&lt;'patt,'expr&gt; - Type of rule. </para>                                              *)
-    (*  <para>  'patt - type of attributes (arguments). </para>                                         *)
-    (*  <para>  'expr - type of expressions in action code. </para>                                     *)
-    (*  <para>Rule have the following format: </para>                                                   *)
-    (*  <para>  [+]name&lt;&lt; metaArgs &gt;&gt;[args] : body; </para>                                 *)
-    (*  </summary>                                                                                      *)
-    type Rule 'patt 'expr = {
-        (*  Rule name. Used to start from this or to be referenced to from other rules.                 *)
-        name    : Source;
-        (*  Heritable arguments of rule                                                                 *)
-        args    : list 'patt;
-        (*  Rule body (production).                                                                     *)
-        body    : Production 'patt 'expr;
-        (*  Is this rule a start non-terminal (in this case '[<Start>]' is used before rule)            *)
-        isStart : bool;
-        (*  Can this rule be seen from another module.                                                  *)
-        (*  It's true if ('public' is used before rule) or (module is marked as AllPublic and rule isn't marked as private)*)
-        isPublic : bool;
-        (*  List of meta-arguments - names of rules, parametrizing this rule.                           *)
-        metaArgs: list 'patt
-    }
 
-    let defaultRule name body = {
-        name = name; 
-        body = body; 
-        args = []; 
-        isStart = false; 
-        isPublic = false; 
-        metaArgs = []
-    }
-//-----------------------------------------------------------------------------------------------------------------
+type rule 'patt 'expr = {
+    (*  Rule name. Used to start from this or to be referenced to from other rules.                 *)
+    name    : source;
+    (*  Heritable arguments of rule                                                                 *)
+    args    : list 'patt;
+    (*  Rule body (Production).                                                                     *)
+    body    : production 'patt 'expr;
+    (*  Is this rule a start non-terminal (in this case '[<Start>]' is used before rule)            *)
+    isStart : bool;
+    (*  Can this rule be seen from another module.                                                  *)
+    (*  It's true if ('public' is used before rule) or (module is marked as AllPublic and rule isn't marked as private)*)
+    isPublic : bool;
+    (*  List of meta-arguments - names of rules, parametrizing this rule.                           *)
+    metaArgs: list 'patt
+}
+assume HasEq_rule: forall a b. hasEq a /\ hasEq b ==> hasEq (rule a b)
 
+let defaultRule name body = {
+    name = name; 
+    body = body; 
+    args = []; 
+    isStart = false; 
+    isPublic = false; 
+    metaArgs = []
+}
 
+(*
 // Grammar
 //-----------------------------------------------------------------------------------------------------------------
-    type Module 'patt 'expr = {
+    type module 'patt 'expr = {
         (*  Module is a list of rules                                                                   *)
         rules : list (Rule 'patt 'expr);
         openings : list Source;
@@ -130,7 +110,7 @@ module IL
         allPublic : bool
     }
     (*  Grammar is a list of modules                                                                    *)
-    type Grammar 'patt 'expr = list (Module 'patt 'expr)
+    type grammar 'patt 'expr = list (module 'patt 'expr)
 //-----------------------------------------------------------------------------------------------------------------
 
 
@@ -160,3 +140,4 @@ module IL
         (*options = Map.empty; *)
         (*tokens = Map.empty*)
     }
+*)
