ToCNF/Yard.Core.Conversions.Helpers.fst
@@ -1,81 +1,98 @@
 module Yard.Core.Conversions.Helpers
     open IL
 
-    val isPToken: Production 'a 'b -> Tot bool
-    let isPToken prod = match prod with PToken(_) -> true | _ -> false
+    val isPToken: #a:Type -> #b:Type
+        -> production a b -> Tot bool
+    let isPToken #a #b prod = match prod with 
+        | PToken(_) -> true 
+        | _ -> false
 
-    val isPRef: Production 'a 'b -> Tot bool
-    let isPRef prod = match prod with PRef(_) -> true | _ -> false
+    val isPRef: #a:Type -> #b:Type
+        -> production a b -> Tot bool
+    let isPRef #a #b prod = match prod with 
+        | PRef(_) -> true 
+        | _ -> false
 
-    val isPSeq: Production 'a 'b -> Tot bool
-    let isPSeq prod = match prod with PSeq(_) -> true | _ -> false
+    val isPSeq: #a:Type -> #b:Type
+        -> production a b -> Tot bool
+    let isPSeq #a #b prod = match prod with 
+        | PSeq(_) -> true 
+        | _ -> false
 
 
-    val isEpsRule: Rule 'a 'b -> Tot bool
-    let isEpsRule rule = match rule.body with PSeq([], _, _) -> true | _ -> false
+    val isEpsRule: #a:Type -> #b:Type
+        -> rule a b -> Tot bool
+    let isEpsRule #a #b rule0 = match rule0.body with 
+        | PSeq([], _, _) -> true 
+        | _ -> false
 
-    val isPTokenRule: rule: Rule 'a 'b {isPSeq rule.body} -> Tot bool
-    let isPTokenRule rule = match rule.body with PSeq(elements,_,_) -> List.length elements = 1 && isPToken (List.Tot.hd elements).rule
+    val isPTokenRule: #a:Type -> #b:Type
+        -> rule0: (rule a b) {isPSeq rule0.body} -> Tot bool
+    let isPTokenRule #a #b rule0 = match rule0.body with 
+        | PSeq(elements,_,_) -> List.Tot.length elements = 1 && isPToken (List.Tot.hd elements).rule
 
 
-    val getLeftPart: rule: Rule 'a 'b -> Tot string
-    let getLeftPart rule = rule.name.text
+    val getLeftPart: #a:Type -> #b:Type
+        -> rule0: rule a b -> Tot string
+    let getLeftPart #a #b rule0 = rule0.name.text
 
-    val getRightPartList: rule: Rule 'a 'b {isPSeq rule.body} -> Tot (list string)
-    let getRightPartList rule = match rule.body with PSeq(elements,_,_) -> 
+    val getRightPartList: #a:Type -> #b:Type
+        -> rule: rule a b {isPSeq rule.body} -> Tot (list string)
+    let getRightPartList #a #b rule = match rule.body with | PSeq(elements,_,_) -> 
             List.Tot.collect (fun elem -> match elem.rule with | PRef(s,_) | PToken(s) -> [s.text] | _ -> []) elements
 
-    val getRightPartPRefList: rule: Rule 'a 'b {isPSeq rule.body} -> Tot (list string)
-    let getRightPartPRefList rule = match rule.body with PSeq(elements,_,_) -> 
-            List.Tot.collect (fun elem -> match elem.rule with PRef(s,_) -> [s.text] | _ -> []) elements
+    val getRightPartPRefList: #a:Type -> #b:Type
+        -> rule: rule a b {isPSeq rule.body} -> Tot (list string)
+    let getRightPartPRefList #a #b rule = match rule.body with | PSeq(elements,_,_) -> 
+            List.Tot.collect (fun elem -> match elem.rule with | PRef(s,_) -> [s.text] | _ -> []) elements
 
 
 //TODO: {isPSeq rule.body}  ------------------------------------------------
-    val getPSeqBodyLength: Production 'a 'b -> Tot nat
-    let getPSeqBodyLength prod = List.length (match prod with PSeq(e, a, l) -> e | _ -> [])
+    val getPSeqBodyLength: #a:Type -> #b:Type 
+        -> production a b -> Tot nat
+    let getPSeqBodyLength #a #b prod = List.Tot.length (match prod with | PSeq(e, a, l) -> e | _ -> [])
 
-    val getRightPartLength: Rule 'a 'b -> Tot nat
-    let getRightPartLength rule = getPSeqBodyLength rule.body
+    val getRightPartLength: #a:Type -> #b:Type
+        -> rule a b -> Tot nat
+    let getRightPartLength #a #b rule = getPSeqBodyLength rule.body
 //------------------------------------------------
 
 
-    val simpleRule: string -> list (elem 'a 'b) -> bool -> Tot (rule: (Rule 'a 'b) {Helpers.isPSeq rule.body})
-    let simpleRule nonTerm seq b =
+    val simpleRule: #a:Type -> #b:Type
+        -> string -> list (elem a b) -> bool -> Tot (rule0: (rule a b) {Helpers.isPSeq rule0.body})
+    let simpleRule #a #b nonTerm seq b =
         {name = new_Source0 nonTerm; args = []; body = PSeq(seq, None, None); isStart = b; isPublic = false; metaArgs = []}
 
-    val simpleStartRule: string -> list (elem 'a 'b) -> Tot (list (rule: (Rule 'a 'b) {Helpers.isPSeq rule.body}))
-    let simpleStartRule nonTerm seq = [simpleRule nonTerm seq true]
+    val simpleStartRule: #a:Type -> #b:Type
+        -> string -> list (elem a b) -> Tot (list (rule0: (rule a b) {Helpers.isPSeq rule0.body}))
+    let simpleStartRule #a #b nonTerm seq = [simpleRule nonTerm seq true]
 
-    val simpleNotStartRule: string -> list (elem 'a 'b) -> Tot (list (rule: (Rule 'a 'b) {Helpers.isPSeq rule.body}))
-    let simpleNotStartRule nonTerm seq = [simpleRule nonTerm seq false]
+    val simpleNotStartRule: #a:Type -> #b:Type
+        -> string -> list (elem a b) -> Tot (list (rule0: (rule a b) {Helpers.isPSeq rule0.body}))
+    let simpleNotStartRule #a #b nonTerm seq = [simpleRule nonTerm seq false]
     
 //------------------------------------------------
 
     // (List.filter f list).length <= list.length
-    val filterLengthLemma: f:('a -> Tot bool) -> l:(list 'a) -> 
+    val filterLengthLemma: #a:eqtype -> f:(a -> Tot bool) -> l:(list a) -> 
         Lemma 
             (requires True) 
-            (ensures (List.length (List.Tot.filter f l)) <= List.length l) 
+            (ensures (List.Tot.length (List.Tot.filter f l)) <= List.Tot.length l) 
             [SMTPat (List.Tot.filter f l)]
-    let rec filterLengthLemma f l = 
+    let rec filterLengthLemma #a f l = 
         match l with  
         | [] -> ()
         | hd::tl -> filterLengthLemma f tl
 
-    val except: list string -> original:list string -> Tot (filtered:list string {List.length filtered <= List.length original}) 
+    val except: list string -> original:list string -> Tot (filtered:list string {List.Tot.length filtered <= List.Tot.length original}) 
     let except itemsToExclude lst = 
         List.Tot.filter (fun el -> not (List.Tot.contains el itemsToExclude)) lst
 
-    val removeDuplicates: list 'a -> Tot (list 'a)
-    let removeDuplicates lst = 
-        let helpRemDup item acc =
-            match acc with 
+    val removeDuplicates: #a:eqtype -> list a -> Tot (list a)
+    let removeDuplicates #a lst = 
+        let helpRemDup item acc = match acc with 
             | [] -> [item]
-            | _ -> if List.existsb (fun x -> x = item) acc then acc else item::acc in 
+            | _ -> if List.Tot.existsb (fun x -> x = item) acc then acc else item::acc in 
         List.Tot.fold_right helpRemDup lst []
 
 
-    val filter: f:('a -> Tot bool) -> list 'a -> Tot (list (m:'a {f m}))
-    let rec filter f = function
-        | [] -> []
-        | hd::tl -> if f hd then hd::filter f tl else filter f tl
