ToCNF/Equ.fst
@@ -1,0 +1,82 @@
+module Equ
+	open FStar.IO
+	open IL
+	open Yard.Core.Conversions
+
+	//let isTerm = Helpers.isPToken
+	//let isNon
+
+	type sentence (patt:eqtype) (expr:eqtype) = terms: list (production patt expr){forall prod. List.Tot.mem prod terms ==> Helpers.isPToken prod}
+	type sententialForm (patt:Type) (expr:Type) = list (production patt expr)
+
+
+
+	val isSentence: #a:eqtype -> #b:eqtype -> list (production a b) -> Tot bool
+	let isSentence #a #b prodList = 
+		List.Tot.for_all Helpers.isPToken prodList
+
+	val str: list (production source source)
+	let str = [PRef (new_Source0 "A", None); PToken (new_Source0 "s")]
+
+
+	val wordE: sentence source source
+	let wordE = [PToken (new_Source0 "1"); PToken (new_Source0 "2")]
+
+
+	//val lderive: #a:Type -> #b:Type -> ruleList: list (rule a b) -> list (production a b) -> int//list (production a b) 
+	//let lderive #a #b ruleList str =
+	//	0
+
+	//val bind: list 'a -> ('a -> Tot (list 'b)) -> Tot (list 'b)
+	//let bind lst f =  
+
+
+	assume val lderives: #a:Type -> #b:Type -> (ruleList: list (rule a b)) -> (oldSF: sententialForm a b) -> (newSF: sententialForm a b) -> Tot bool
+	assume val getStartNonterm: #a:Type -> #b:Type -> list (rule a b) -> Tot (sententialForm a b)
+
+
+
+
+	type language (a:eqtype) (b:eqtype) (ruleList: list (rule a b)) = 
+		lang: list (sentence a b) {forall sent. List.Tot.mem sent lang ==> lderives ruleList (getStartNonterm ruleList) sent}
+
+	assume val transformation: #a:eqtype -> #b:eqtype
+		-> list (rule a b) -> Tot (list (rule a b))
+
+    assume val lemma0: 
+    	#a:eqtype -> #b:eqtype
+		-> ruleList: list (rule a b) -> l1: language a b ruleList -> l2: language a b (transformation ruleList)
+        -> Lemma 
+            (requires True) 
+            (ensures (forall x. List.Tot.mem x l1 ==> List.Tot.mem x l2)) 
+
+    assume val lemma1: 
+    	#a:eqtype -> #b:eqtype
+		-> ruleList: list (rule a b) -> l1: language a b ruleList -> l2: language a b (transformation ruleList)
+        -> Lemma 
+            (requires True) 
+            (ensures (forall x. List.Tot.mem x l2 ==> List.Tot.mem x l1)) 
+
+		
+
+
+
+
+
+    let main = 
+    	//assert (isSentence wordE);
+    	//assert (isSentence str);
+
+    	0
+
+
+ 	
+//	val test: list (rule0: (rule source source) {Helpers.isPSeq rule0.body}) 
+//	let test = (Helpers.simpleStartRule "S" (List.Tot.map create [PRef (new_Source0 "A", None); PToken (new_Source0 "s")]))
+//	    @ (Helpers.simpleNotStartRule "A" (List.Tot.map create [PRef (new_Source0 "B", None)]))
+//	    @ (Helpers.simpleNotStartRule "B" (List.Tot.map create [PRef (new_Source0 "C", None)]))
+//	    @ (Helpers.simpleNotStartRule "C" (List.Tot.map create [PToken (new_Source0 "c")]))
+//	    @ (Helpers.simpleNotStartRule "C" (List.Tot.map create [])) 
+
+	//nlist?? = list non_terminal
+
